pcuic/theories/Conversion/PCUICInstConv.v
@@ -295,7 +295,7 @@ Proof.
   - unfold inst_context, snoc. rewrite fold_context_k_snoc0.
     unfold snoc. f_equal. all: auto.
     unfold map_decl. simpl. unfold vass. f_equal.
-    destruct t0 as [s ht]. eapply typed_inst. all: eauto.
+    destruct t0 as [s [e ht]]. eapply typed_inst. all: eauto.
   - unfold inst_context, snoc. rewrite fold_context_k_snoc0.
     unfold snoc. f_equal. all: auto.
     unfold map_decl. simpl. unfold vdef. f_equal.
@@ -1611,14 +1611,16 @@ Proof.
   intros.
   induction X.
   - now simpl.
-  - simpl. destruct t0 as [s Hs].
+  - simpl. destruct t0 as [s [e Hs]].
     rewrite inst_context_snoc /=. constructor; auto.
     red. simpl. exists s.
+    split; [apply e | idtac].
     eapply (Hs (Δ' ,,, inst_context σ Γ0) (⇑^#|Γ0| σ)) => //.
     eapply well_subst_app; auto.
-  - simpl. destruct t0 as [s Hs]. simpl in t1.
+  - simpl. destruct t0 as [s [e Hs]]. simpl in t1.
     rewrite inst_context_snoc /=. constructor; auto.
     * simpl. exists s.
+      split; [apply e | idtac].
       eapply (Hs (Δ' ,,, inst_context σ Γ0) (⇑^#|Γ0| σ)) => //.
       eapply well_subst_app; auto.
     * simpl. apply t1 => //.
