pcuic/theories/Conversion/PCUICWeakeningEnvConv.v
@@ -240,8 +240,8 @@ Lemma extends_wf_local `{checker_flags} Σ Γ (wfΓ : wf_local Σ Γ) :
 Proof.
   intros X0 Σ' H0.
   induction X0 in H0 |- *; try econstructor; simpl in *; intuition auto.
-  - destruct tu as [u Hu]; exists u; auto.
-  - destruct tu as [u Hu]; exists u; auto.
+  - destruct tu as [u [e Hu]]; exists u; auto.
+  - destruct tu as [u [e Hu]]; exists u; auto.
 Qed.
 #[global]
 Hint Resolve extends_wf_local : extends.
@@ -412,7 +412,7 @@ Qed.
 Hint Resolve weakening_env_is_allowed_elimination : extends.
 
 Lemma weakening_All_local_env_impl `{checker_flags}
-      (P Q : context -> term -> option term -> Type) l :
+      (P Q : context -> term -> typ_or_rel_or_none -> Type) l :
   All_local_env P l ->
   (forall Γ t T, P Γ t T -> Q Γ t T) ->
   All_local_env Q l.
@@ -640,11 +640,11 @@ Proof.
 Qed.
 
 Definition weaken_env_prop `{checker_flags}
-           (P : global_env_ext -> context -> term -> option term -> Type) :=
+           (P : global_env_ext -> context -> term -> typ_or_rel_or_none -> Type) :=
   forall Σ Σ' φ, wf Σ -> wf Σ' -> extends Σ Σ' -> forall Γ t T, P (Σ, φ) Γ t T -> P (Σ', φ) Γ t T.
 
 Definition weaken_env_decls_prop `{checker_flags}
-  (P : global_env_ext -> context -> term -> option term -> Type) :=
+  (P : global_env_ext -> context -> term -> typ_or_rel_or_none -> Type) :=
   forall Σ Σ' φ, wf Σ' -> extends_decls Σ Σ' -> forall Γ t T, P (Σ, φ) Γ t T -> P (Σ', φ) Γ t T.
 
 Lemma extends_decls_wf {cf} Σ Σ' : 
