pcuic/theories/PCUICArities.v
@@ -77,7 +77,7 @@ Proof.
   (Σ, ind_universes mdecl) ;;; [] |- tInd {| inductive_mind := inductive_mind ind; inductive_ind := i |} u : (ind_type x)) 0 (ind_bodies mdecl)).
   { apply forall_nth_error_Alli. intros.
     eapply Alli_nth_error in oind; eauto. simpl in oind.
-    destruct oind. destruct onArity as [s Hs].
+    destruct oind. destruct onArity as [s [e Hs]].
     eapply type_Cumul; eauto.
     econstructor; eauto. split; eauto with pcuic.
     eapply consistent_instance_ext_abstract_instance; eauto.
@@ -205,17 +205,19 @@ Section WfEnv.
   Qed.
 
   Lemma isType_tProd {Γ} {na A B} : 
-    isType Σ Γ (tProd na A B) <~> (isType Σ Γ A × isType Σ (Γ,, vass na A) B).
+    isType Σ Γ (tProd na A B) <~> (isTypeRel Σ Γ A na.(binder_relevance) × isType Σ (Γ,, vass na A) B).
   Proof.
     split; intro HH.
     - destruct HH as [s H].
-      apply inversion_Prod in H; tas. destruct H as [s1 [s2 [HA [HB Hs]]]].
+      apply inversion_Prod in H; tas. destruct H as [s1 [s2 [e' [HA [HB Hs]]]]].
       split.
-      * eexists; tea.
+      * eexists; split; eauto.
       * eexists; tea.
     - destruct HH as [HA HB].
-      destruct HA as [sA HA], HB as [sB HB].
-      eexists. econstructor; eassumption.
+      destruct HA as [sA [e HA]], HB as [sB HB].
+      exists (Universe.sort_of_product sA sB).
+      destruct na; cbn in e |- *; rewrite <- e in HB |- *.
+      econstructor; eassumption.
   Defined.
 
   Lemma isType_subst {Γ Δ A} s :
@@ -257,7 +259,7 @@ Section WfEnv.
     destruct HH as [s H].
     exists s.
     assert (Hs := typing_wf_universe _ H).
-    apply inversion_LetIn in H; tas. destruct H as [s1 [A' [HA [Ht [HB H]]]]].
+    apply inversion_LetIn in H; tas. destruct H as [s1 [A' [e [HA [Ht [HB H]]]]]].
     eapply (type_ws_cumul_pb (pb:=Cumul)) with (A' {0 := t}). eapply substitution_let in HB; eauto.
     * econstructor; eauto with pcuic. econstructor; eauto.
     * eapply ws_cumul_pb_Sort_r_inv in H as [s' [H H']].
@@ -274,12 +276,12 @@ Section WfEnv.
   Proof.
     intro HH.
     destruct HH as [s H].
-    apply inversion_LetIn in H; tas. now destruct H as [s1 [A' [HA [Ht [HB H]]]]].
+    apply inversion_LetIn in H; tas. now destruct H as [s1 [A' [e [HA [Ht [HB H]]]]]].
   Qed.
 
   Lemma wf_local_ass {Γ na A} : 
     wf_local Σ Γ ->
-    isType Σ Γ A ->
+    isTypeRel Σ Γ A na.(binder_relevance) ->
     wf_local Σ (Γ ,, vass na A).
   Proof.
     constructor; eauto with pcuic.
@@ -287,7 +289,7 @@ Section WfEnv.
 
   Lemma wf_local_def {Γ na d ty} : 
     wf_local Σ Γ ->
-    isType Σ Γ ty ->
+    isTypeRel Σ Γ ty na.(binder_relevance) ->
     Σ ;;; Γ |- d : ty ->
     wf_local Σ (Γ ,, vdef na d ty).
   Proof.
@@ -382,7 +384,8 @@ Section WfEnv.
     induction 1; auto.
   Qed.
 
-  Lemma type_mkProd_or_LetIn {Γ} d {u t s} : 
+  Lemma type_mkProd_or_LetIn {Γ} d {u t s} :
+    relevance_of_sort u = d.(decl_name).(binder_relevance) ->
     Σ ;;; Γ |- decl_type d : tSort u ->
     Σ ;;; Γ ,, d |- t : tSort s ->
     match decl_body d return Type with 
@@ -390,14 +393,18 @@ Section WfEnv.
     | None => Σ ;;; Γ |- mkProd_or_LetIn d t : tSort (Universe.sort_of_product u s)
     end.
   Proof.
-    destruct d as [na [b|] dty] => [Hd Ht|Hd Ht]; rewrite /mkProd_or_LetIn /=.
+    destruct d as [na [b|] dty] => [e Hd Ht|e Hd Ht]; rewrite /mkProd_or_LetIn /=.
     - have wf := typing_wf_local Ht.
       depelim wf. clear l.
-      eapply type_Cumul. econstructor; eauto.
+      eapply type_Cumul.
+      destruct na; cbn in e; rewrite <- e in Ht |- *.
+      econstructor; eauto.
       econstructor; eauto. now eapply typing_wf_universe in Ht; pcuic.
       eapply convSpec_cumulSpec, red1_cumulSpec. constructor.
     - have wf := typing_wf_local Ht.
       depelim wf; clear l.
+      cbn in Hd.
+      destruct na; cbn in e; rewrite <- e in Ht |- *.
       eapply type_Prod; eauto.
   Qed.
 
@@ -421,7 +428,8 @@ Section WfEnv.
       destruct a as [na [b|] ty]; intuition auto.
       { apply typing_wf_local in Ht as XX. inversion XX; subst.
         eapply (type_mkProd_or_LetIn {| decl_body := Some b |}); auto.
-        + simpl. exact X0.π2.
+        + simpl. exact X0.π2.1.
+        + simpl. exact X0.π2.2.
         + eapply type_Cumul; eauto.
           econstructor; eauto with pcuic.
           eapply cumul_Sort. eapply leq_universe_product. }
@@ -457,11 +465,12 @@ Section WfEnv.
     induction Γ'; simpl; auto; move=> Γ us s t equ Ht.
     - destruct us => //.
     - destruct a as [na [b|] ty]; intuition auto.
-      * destruct a0 as [s' Hs].
+      * destruct a0 as [s' [e Hs]].
         eapply IHΓ'; eauto.
         eapply (type_mkProd_or_LetIn {| decl_body := Some b |}); auto.
+        apply e.
         simpl. exact Hs.
-      * destruct us => //. destruct equ.
+      * destruct us => //. destruct equ as [s0 [e p]].
         simpl.   
         eapply IHΓ'; eauto.
         apply (type_mkProd_or_LetIn {| decl_body := None |}) => /=; eauto.
@@ -604,7 +613,7 @@ Section WfEnv.
       
       intros Hs.
       assert (wfs' := typing_wf_universe wfΣ Hs).
-      eapply inversion_LetIn in Hs as [? [? [? [? [? ?]]]]]; auto.
+      eapply inversion_LetIn in Hs as [? [? [? [? [? [? ?]]]]]]; auto.
       eapply substitution_let in t1; auto.
       eapply ws_cumul_pb_LetIn_l_inv in w; auto.
       pose proof (subslet_app_inv sub) as [subl subr].
@@ -620,7 +629,7 @@ Section WfEnv.
       
       intros Hs.
       assert (wfs' := typing_wf_universe wfΣ Hs).
-      eapply inversion_Prod in Hs as [? [? [? [? ?]]]]; auto.
+      eapply inversion_Prod in Hs as [? [? [? [? [? ?]]]]]; auto.
       pose proof (subslet_app_inv sub) as [subl subr].
       depelim subl; depelim subl. rewrite subst_empty in t2. rewrite H0 in subr.
       epose proof (substitution0 t0 t2).
@@ -656,14 +665,14 @@ Section WfEnv.
     + simpl. intros. now eapply typing_wf_local in X.
     + rewrite it_mkProd_or_LetIn_app.
       destruct x as [na [b|] ty]; cbn; move=> H.
-      * apply inversion_LetIn in H as (s1 & A & H0 & H1 & H2 & H3); auto.
+      * apply inversion_LetIn in H as (s1 & A & e & H0 & H1 & H2 & H3); auto.
         eapply All_local_env_app; split; pcuic.
         eapply All_local_env_app. split. repeat constructor. now exists s1.
         auto. apply IHΔ in H2.
         eapply All_local_env_app_inv in H2. intuition auto.
         eapply All_local_env_impl; eauto. simpl. intros.
         now rewrite app_context_assoc.
-      * apply inversion_Prod in H as (s1 & A & H0 & H1 & H2); auto.
+      * apply inversion_Prod in H as (s1 & A & e & H0 & H1 & H2); auto.
         eapply All_local_env_app; split; pcuic. 
         eapply All_local_env_app. split. repeat constructor. now exists s1.
         apply IHΔ in H1.
